Continue

src/Suc_Theory.thy
@@ -1,65 +1,103 @@
 theory Suc_Theory
-  imports Main "HOL-Library.Adhoc_Overloading"
+  imports Main "HOL-Library.Adhoc_Overloading" Fresh_Identifiers.Fresh
 begin
 
-datatype 'a suc_term = Var 'a | Succ nat "'a suc_term"
+datatype 'a suc_term = Var 'a | Zero | Succ nat "'a suc_term"
 
-datatype 'a suc_atom = Eq "'a suc_term" "'a suc_term"
+datatype 'a suc_atom = is_Eq: Eq "'a suc_term" "'a suc_term" | is_NEq: NEq "'a suc_term" "'a suc_term"
 
 fun succ :: "nat \<Rightarrow> 'a suc_term \<Rightarrow> 'a suc_term" where
   "succ n (Succ k t) = succ (n + k) t"
 | "succ 0 t = t"
-| "succ n (Var x) = Succ n (Var x)"
+| "succ n t = Succ n t"
 
-fun is_normal_term :: "'a suc_term \<Rightarrow> bool" where
-  "is_normal_term (Var _) \<longleftrightarrow> True"
-| "is_normal_term (Succ n (Var _)) \<longleftrightarrow> n \<noteq> 0"
-| "is_normal_term (Succ _ (Succ _ _)) \<longleftrightarrow> False"
+fun is_suc_normal_term :: "'a suc_term \<Rightarrow> bool" where
+  "is_suc_normal_term (Var _) \<longleftrightarrow> True"
+| "is_suc_normal_term Zero \<longleftrightarrow> True"
+| "is_suc_normal_term (Succ n Zero) \<longleftrightarrow> n \<noteq> 0"
+| "is_suc_normal_term (Succ n (Var _)) \<longleftrightarrow> n \<noteq> 0"
+| "is_suc_normal_term (Succ _ (Succ _ _)) \<longleftrightarrow> False"
 
-fun is_normal_atom :: "'a suc_atom \<Rightarrow> bool" where
-  "is_normal_atom (Eq t1 t2) \<longleftrightarrow> is_normal_term t1 \<and> is_normal_term t2"
+fun is_suc_normal_atom :: "'a suc_atom \<Rightarrow> bool" where
+  "is_suc_normal_atom (Eq t1 t2) \<longleftrightarrow> is_suc_normal_term t1 \<and> is_suc_normal_term t2"
+| "is_suc_normal_atom (NEq t1 t2) \<longleftrightarrow> is_suc_normal_term t1 \<and> is_suc_normal_term t2"
 
-consts is_normal :: "'a \<Rightarrow> bool"
-adhoc_overloading is_normal is_normal_term is_normal_atom
+consts is_suc_normal :: "'a \<Rightarrow> bool"
+adhoc_overloading is_suc_normal is_suc_normal_term is_suc_normal_atom
 
-fun I_suc_term :: "('a \<Rightarrow> nat) \<Rightarrow> 'a suc_term \<Rightarrow> nat" where
-  "I_suc_term v (Var x) = v x"
-| "I_suc_term v (Succ n t) = (Suc ^^ n) (I_suc_term v t)"
+fun is_Zero_free_term :: "'a suc_term \<Rightarrow> bool" where
+  "is_Zero_free_term (Var _) \<longleftrightarrow> True"
+| "is_Zero_free_term Zero \<longleftrightarrow> False"
+| "is_Zero_free_term (Succ _ t) \<longleftrightarrow> is_Zero_free_term t"
 
-fun I_suc_atom :: "('a \<Rightarrow> nat) \<Rightarrow> 'a suc_atom \<Rightarrow> bool" where
-  "I_suc_atom v (Eq t1 t2) \<longleftrightarrow> I_suc_term v t1 = I_suc_term v t2"
+fun is_Zero_free_atom :: "'a suc_atom \<Rightarrow> bool" where
+  "is_Zero_free_atom (Eq t1 t2) \<longleftrightarrow> is_Zero_free_term t1 \<and> is_Zero_free_term t2"
+| "is_Zero_free_atom (NEq t1 t2) \<longleftrightarrow> is_Zero_free_term t1 \<and> is_Zero_free_term t2"
 
-fun subst_suc_term :: "('a \<Rightarrow> 'a suc_term) \<Rightarrow> 'a suc_term \<Rightarrow> 'a suc_term" where
-  "subst_suc_term \<sigma> (Var x) = succ 0 (\<sigma> x)"
-| "subst_suc_term \<sigma> (Succ n t) = succ n (subst_suc_term \<sigma> t)"
+consts is_Zero_free :: "'a \<Rightarrow> bool"
+adhoc_overloading is_Zero_free is_Zero_free_term is_Zero_free_atom
 
-fun subst_suc_atom :: "('a \<Rightarrow> 'a suc_term) \<Rightarrow> 'a suc_atom \<Rightarrow> 'a suc_atom" where
-  "subst_suc_atom \<sigma> (Eq t1 t2) = Eq (subst_suc_term \<sigma> t1) (subst_suc_term \<sigma> t2)"
+fun I_term :: "('a \<Rightarrow> nat) \<Rightarrow> 'a suc_term \<Rightarrow> nat" where
+  "I_term v (Var x) = v x"
+| "I_term v Zero = 0"
+| "I_term v (Succ n t) = (Suc ^^ n) (I_term v t)"
 
-lemma I_suc_term_succ: "I_suc_term v (succ n t) = I_suc_term v (Succ n t)"
+fun I_atom :: "('a \<Rightarrow> nat) \<Rightarrow> 'a suc_atom \<Rightarrow> bool" where
+  "I_atom v (Eq t1 t2) \<longleftrightarrow> I_term v t1 = I_term v t2"
+| "I_atom v (NEq t1 t2) \<longleftrightarrow> I_term v t1 \<noteq> I_term v t2"
+
+fun subst_term :: "('a \<Rightarrow> 'a suc_term) \<Rightarrow> 'a suc_term \<Rightarrow> 'a suc_term" where
+  "subst_term \<sigma> (Var x) = succ 0 (\<sigma> x)"
+| "subst_term _ Zero = Zero"
+| "subst_term \<sigma> (Succ n t) = succ n (subst_term \<sigma> t)"
+
+fun subst_atom :: "('a \<Rightarrow> 'a suc_term) \<Rightarrow> 'a suc_atom \<Rightarrow> 'a suc_atom" where
+  "subst_atom \<sigma> (Eq t1 t2) = Eq (subst_term \<sigma> t1) (subst_term \<sigma> t2)"
+| "subst_atom \<sigma> (NEq t1 t2) = NEq (subst_term \<sigma> t1) (subst_term \<sigma> t2)"
+
+lemma I_term_succ: "I_term v (succ n t) = I_term v (Succ n t)"
   apply(induction n t rule: succ.induct)
     apply(auto)
   done
 
-lemma is_normal_succ[simp]: "is_normal (succ n t)"
+lemma is_suc_normal_succ[simp]: "is_suc_normal (succ n t)"
   apply(induction n t rule: succ.induct)
     apply(auto)
   done
 
-lemma is_normal_subst_suc_term[simp]: "is_normal (subst_suc_term \<sigma> t)"
+lemma is_suc_normal_subst_term[simp]: "is_suc_normal (subst_term \<sigma> t)"
   apply(induction t)
    apply(auto)
   done
 
-lemma is_normal_subst_suc_atom[simp]: "is_normal (subst_suc_atom \<sigma> a)"
-  by (cases a) simp
+lemma is_suc_normal_subst_atom[simp]: "is_suc_normal (subst_atom \<sigma> a)"
+  by (cases a) simp_all
+
+lemma is_Zero_free_succ[simp]: "is_Zero_free (succ n t) = is_Zero_free t"
+  apply(induction n t rule: succ.induct)
+      apply(auto)
+  done
+
+lemma is_Zero_free_subst_term[simp]:
+  "is_Zero_free t \<Longrightarrow> is_Zero_free (subst_term (Var(x := t)) s) \<longleftrightarrow> is_Zero_free s"
+  apply(induction s)
+    apply(auto)
+  done
+
+lemma is_Zero_free_subst_atom[simp]:
+  "is_Zero_free t \<Longrightarrow> is_Zero_free (subst_atom (Var(x := t)) a) \<longleftrightarrow> is_Zero_free a"
+  by (cases a) auto
+
+lemma is_NEq_subst_atom[simp]:
+  "is_NEq (subst_atom v a) \<longleftrightarrow> is_NEq a"
+  by (cases a) auto
 
 abbreviation solve_Var_Eq_Succ where
 "solve_Var_Eq_Succ solve x n y es \<equiv>
     (if x = y
       then (if n = 0 then solve es else None)
       else map_option ((#) (Eq (Var x) (succ n (Var y))))
-            (solve (map (subst_suc_atom (Var(x := succ n (Var y)))) es))
+            (solve (map (subst_atom (Var(x := succ n (Var y)))) es))
     )"
 
 fun solve :: "'a suc_atom list \<Rightarrow> 'a suc_atom list option" where
@@ -67,7 +105,7 @@ fun solve :: "'a suc_atom list \<Rightarrow> 'a suc_atom list option" where
 | "solve (Eq (Var x) (Var y) # es) =
     (if x = y
       then solve es
-      else map_option ((#) (Eq (Var x) (Var y))) (solve (map (subst_suc_atom (Var(x := Var y))) es))
+      else map_option ((#) (Eq (Var x) (Var y))) (solve (map (subst_atom (Var(x := Var y))) es))
     )"
 | "solve (Eq (Var x) (Succ n (Var y)) # es) = solve_Var_Eq_Succ solve x n y es"
 | "solve (Eq (Succ n (Var y)) (Var x) # es) = solve_Var_Eq_Succ solve x n y es"
@@ -77,83 +115,371 @@ fun solve :: "'a suc_atom list \<Rightarrow> 'a suc_atom list option" where
       else solve_Var_Eq_Succ solve x (k - n) y es
     )"
 
-lemma is_normal_solve:
+abbreviation "is_normal a \<equiv> \<not> is_NEq a \<and> is_Zero_free a \<and> is_suc_normal a"
+
+lemma is_suc_normal_solve:
   assumes "solve es = Some ss" "\<forall>a \<in> set es. is_normal a"
   assumes "a \<in> set ss"
-  shows "is_normal a"
+  shows "is_suc_normal a"
   using assms
   apply(induction es arbitrary: ss rule: solve.induct)
             apply(auto split: if_splits)
   done
 
-lemma I_suc_term_subst_suc_term:
-  assumes "I_suc_atom v (Eq (Var x) t)"
-  shows "I_suc_term v (subst_suc_term (Var(x := t)) s) = I_suc_term v s"
+lemma I_term_subst_term:
+  assumes "I_atom v (Eq (Var x) t)"
+  shows "I_term v (subst_term (Var(x := t)) s) = I_term v s"
   using assms
   apply(induction s)
-   apply(auto simp: I_suc_term_succ)
+   apply(auto simp: I_term_succ)
   done
 
-lemma I_suc_atom_subst_suc_atom:
-  assumes "I_suc_atom v (Eq (Var x) t)"
-  shows "I_suc_atom v (subst_suc_atom (Var(x := t)) a) \<longleftrightarrow> I_suc_atom v a"
+lemma I_atom_subst_atom:
+  assumes "I_atom v (Eq (Var x) t)"
+  shows "I_atom v (subst_atom (Var(x := t)) a) \<longleftrightarrow> I_atom v a"
   using assms
-  by (cases a) (auto simp: I_suc_term_subst_suc_term)
+  by (cases a) (auto simp: I_term_subst_term)
 
-lemma I_suc_atom_sym: "I_suc_atom v (Eq s t) \<longleftrightarrow> I_suc_atom v (Eq t s)"
-  by auto
-
-lemma I_suc_atom_solve_Some:
-  assumes "solve es = Some ss" "\<forall>a \<in> set es. is_normal a" "\<forall>a \<in> set es. I_suc_atom v a"
-  assumes "a \<in> set ss"
-  shows "I_suc_atom v a"
-  using assms
-  apply(induction es arbitrary: ss rule: solve.induct)
-            apply(auto simp: I_suc_atom_subst_suc_atom I_suc_term_succ split: if_splits)
-  done
-
-lemma I_suc_atom_solve_None:
+lemma I_atom_solve_None:
   assumes "solve es = None" "\<forall>a \<in> set es. is_normal a"
-  shows "\<exists>a \<in> set es. \<not> I_suc_atom v a"
+  shows "\<exists>a \<in> set es. \<not> I_atom v a"
 proof -
-  have "False" if "\<forall>a \<in> set es. I_suc_atom v a"
+  have "False" if "\<forall>a \<in> set es. I_atom v a"
     using assms that
     apply(induction es rule: solve.induct)
-              apply(auto simp: I_suc_atom_subst_suc_atom I_suc_term_succ split: if_splits)
+              apply(auto simp: I_atom_subst_atom I_term_succ split: if_splits)
     done
   then show ?thesis
     by blast
 qed
 
-lemma
-  assumes "\<forall>v. \<exists>a \<in> set es. \<not> I_suc_atom v a" "\<forall>a \<in> set es. is_normal a"
-  shows "solve es = None"
+lemma set_suc_term_succ[simp]: "set_suc_term (succ n t) = set_suc_term t"
+  by (induction n t rule: succ.induct) auto
+
+lemma not_mem_subst_term_self:
+  assumes "x \<notin> set_suc_term t"
+  shows "x \<notin> set_suc_term (subst_term (Var(x := t)) s)"
   using assms
-proof(induction es rule: solve.induct)
+  apply(induction s)
+   apply(auto)
+  done
+
+lemma not_mem_subst_atom_self:
+  assumes "x \<notin> set_suc_term t"
+  shows "x \<notin> set_suc_atom (subst_atom (Var(x := t)) a)"
+  using not_mem_subst_term_self[OF assms] by (cases a) simp_all
+
+lemma not_mem_subst_term:
+  assumes "z \<notin> set_suc_term t" "z \<notin> set_suc_term s"
+  shows "z \<notin> set_suc_term (subst_term (Var(x := t)) s)"
+  using assms 
+  apply(induction s)
+   apply(auto)
+  done
+
+lemma not_mem_subst_atom:
+  assumes "z \<notin> set_suc_term t" "z \<notin> set_suc_atom a"
+  shows "z \<notin> set_suc_atom (subst_atom (Var(x := t)) a)"
+  using not_mem_subst_term[OF assms(1)] assms(2) by (cases a) simp_all
+
+lemma not_mem_suc_atom_solve:
+  assumes "solve es = Some ss" "\<forall>a \<in> set es. is_normal a"
+  assumes "\<forall>a \<in> set es. z \<notin> set_suc_atom a"
+  shows "\<forall>a \<in> set ss. z \<notin> set_suc_atom a"
+  using assms
+  apply(induction es arbitrary: ss rule: solve.induct)
+            apply(auto simp: not_mem_subst_atom split: if_splits)
+  done
+
+lemma not_mem_suc_atom_if_solve:
+  assumes "solve es = Some (Eq (Var x) t # ss)" "\<forall>a \<in> set es. is_normal a"
+  shows "\<forall>a \<in> set ss. x \<notin> set_suc_atom a"
+  using assms
+proof(induction es arbitrary: ss rule: solve.induct)
   case (2 x y es)
-  then show ?case apply(auto split: if_splits) sorry
+  note not_mem_suc_atom_solve[where ?es="map (subst_atom (Var(x := Var y))) es" and ?z=x]
+  with 2 show ?case
+    by (auto simp: not_mem_subst_atom_self split: if_splits)
 next
   case (3 x n y es)
-  then show ?case sorry
-next
+  note not_mem_suc_atom_solve[
+      where ?es="map (subst_atom (Var(x := succ n (Var y)))) es" and ?z=x]
+  with 3 show ?case
+    by (auto simp: not_mem_subst_atom_self split: if_splits)
+next                                          
   case (4 n y x es)
-  then show ?case sorry
+  note not_mem_suc_atom_solve[
+      where ?es="map (subst_atom (Var(x := succ n (Var y)))) es" and ?z=x]
+  with 4 show ?case
+    by (auto simp: not_mem_subst_atom_self split: if_splits)
 next
   case (5 n x k y es)
-  then show ?case sorry
+  note not_mem_suc_atom_solve[
+      where ?es="map (subst_atom (Var(y := succ (n - k) (Var x)))) es" and ?z=y]
+   and not_mem_suc_atom_solve[
+      where ?es="map (subst_atom (Var(x := succ (k - n) (Var y)))) es" and ?z=x]
+  with 5 show ?case
+    by (auto simp: not_mem_subst_atom_self split: if_splits)
 qed auto
 
+fun assign :: "'a suc_atom list \<Rightarrow> ('a \<Rightarrow> nat)" where
+  "assign [] = (\<lambda>x. 0)"
+| "assign (Eq (Var x) (Var y) # ss) = (let ass = assign ss in ass(x := ass y))"
+| "assign (Eq (Var x) (Succ n (Var y)) # ss) = (let ass = assign ss in ass(x := (Suc^^n) (ass y)))"
 
+lemma assign_succ:
+  "assign (Eq (Var x) (succ n (Var y)) # ss) = assign (Eq (Var x) (Succ n (Var y)) # ss)"
+  apply(cases "(n, Var y)" rule: succ.cases)
+    apply(auto)
+  done
+
+lemma I_term_fun_upd:
+  assumes "x \<notin> set_suc_term t"
+  shows "I_term (v(x := s)) t = I_term v t"
+  using assms apply(induction t) apply(auto) done
+
+lemma I_atom_fun_upd:
+  assumes "x \<notin> set_suc_atom a"
+  shows "I_atom (v(x := s)) a = I_atom v a"
+  using assms apply (cases a) apply(auto simp: I_term_fun_upd) done
+
+lemma I_atom_fun_updI:
+  assumes "x \<notin> set_suc_atom a" "I_atom v a"
+  shows "I_atom (v(x := s)) a"
+  using assms I_atom_fun_upd by metis
+
+lemma I_atom_assign_if_solve:
+  assumes "solve es = Some ss" "\<forall>a \<in> set es. is_normal a"
+  shows "\<forall>a \<in> set ss. I_atom (assign ss) a"
+  using assms
+proof(induction es arbitrary: ss rule: solve.induct)
+  case (2 x y es)
+  note not_mem_suc_atom_if_solve[where ?es="Eq (Var x) (Var y) # es" and ?x=x]
+  with 2 show ?case
+    by (auto simp: Let_def I_atom_fun_upd split: if_splits)
+next
+  case (3 x n y es)
+  note not_mem_suc_atom_if_solve[where ?es="Eq (Var x) (Succ n (Var y)) # es" and ?x=x]
+  with 3 show ?case
+    by (auto simp: Let_def I_term_succ I_atom_fun_upd assign_succ split: if_splits)
+next
+  case (4 n y x es)
+  note not_mem_suc_atom_if_solve[where ?es="Eq (Var x) (Succ n (Var y)) # es" and ?x=x]
+  with 4 show ?case
+    by (auto simp: Let_def I_term_succ I_atom_fun_upd assign_succ split: if_splits)
+next
+  case (5 n x k y es)
+  note not_mem_suc_atom_if_solve[where ?es="Eq (Succ n (Var x)) (Succ k (Var y)) # es" and ?x=x]
+   and not_mem_suc_atom_if_solve[where ?es="Eq (Succ n (Var x)) (Succ k (Var y)) # es" and ?x=y]
+  with 5 show ?case
+    by (auto simp: Let_def I_term_succ I_atom_fun_upd assign_succ split: if_splits)
+qed auto
+
+lemma I_atom_if_I_atom_solve:
+  assumes "solve es = Some ss" "\<forall>a \<in> set es. is_normal a"
+  assumes "\<forall>a \<in> set ss. I_atom v a"
+  shows "\<forall>a \<in> set es. I_atom v a"
+  using assms
+proof(induction es arbitrary: ss rule: solve.induct)
+  case (2 x y es)
+  then show ?case
+    by (auto simp: I_atom_subst_atom split: if_splits)
+next
+  case (3 x n y es)
+  then show ?case
+    by (auto simp: I_term_succ I_atom_subst_atom split: if_splits)
+next
+  case (4 n y x es)
+  then show ?case
+    by (auto simp: I_term_succ I_atom_subst_atom split: if_splits)
+next
+  case (5 n x k y es)
+  from "5"(1,2,4-) show ?case
+    by (auto simp: I_term_succ I_atom_subst_atom split: if_splits)
+qed auto
+
+lemma assign_minimal_if_solve:
+  assumes "solve es = Some ss" "\<forall>a \<in> set es. is_normal a"
+  assumes "\<forall>a \<in> set ss. I_atom v a"
+  shows "assign ss z \<le> v z"
+  using assms
+proof(induction es arbitrary: ss z rule: solve.induct)
+  case (2 x y es)
+  note not_mem_suc_atom_if_solve[where ?es="Eq (Var x) (Var y) # es" and ?x=x]
+  with 2 show ?case
+    by (auto simp: Let_def split: if_splits)
+next
+  case (3 x n y es)
+  note not_mem_suc_atom_if_solve[where ?es="Eq (Var x) (Succ n (Var y)) # es" and ?x=x]
+  with 3 show ?case
+    by (auto simp: Let_def I_term_succ assign_succ split: if_splits)
+next
+  case (4 n y x es)
+  note not_mem_suc_atom_if_solve[where ?es="Eq (Var x) (Succ n (Var y)) # es" and ?x=x]
+  with 4 show ?case
+    by (auto simp: Let_def I_term_succ assign_succ split: if_splits)
+next
+  case (5 n x k y es)
+  note not_mem_suc_atom_if_solve[where ?es="Eq (Succ n (Var x)) (Succ k (Var y)) # es" and ?x=x]
+   and not_mem_suc_atom_if_solve[where ?es="Eq (Succ n (Var x)) (Succ k (Var y)) # es" and ?x=y]
+  with 5 show ?case
+    by (auto simp: Let_def I_term_succ assign_succ diff_le_mono split: if_splits)
+qed auto
+
+fun elim_NEq_Zero_aux :: "('a::fresh) set \<Rightarrow> 'a suc_atom list \<Rightarrow> 'a suc_atom list" where
+  "elim_NEq_Zero_aux _ [] = []"
+| "elim_NEq_Zero_aux us (NEq (Var x) Zero # es) =
+    (let fx = fresh us x in Eq (Var x) (Succ 1 (Var fx)) # elim_NEq_Zero_aux (insert fx us) es)"
+| "elim_NEq_Zero_aux us (e # es) = e # elim_NEq_Zero_aux us es"
+
+definition elim_NEq_Zero :: "('a::fresh) suc_atom list \<Rightarrow> 'a suc_atom list"
+  where "elim_NEq_Zero es \<equiv> elim_NEq_Zero_aux (\<Union>(set_suc_atom ` set es)) es"
+
+lemma is_normal_elim_NEq_Zero_aux:
+  assumes "\<forall>a \<in> set es. is_Eq a \<longrightarrow> is_normal a"
+  assumes "\<forall>a \<in> set es. is_NEq a \<longrightarrow> (\<exists>x. a = NEq (Var x) Zero)"
+  shows "\<forall>a \<in> set (elim_NEq_Zero_aux us es). is_normal a"
+  using assms
+  apply(induction es rule: elim_NEq_Zero_aux.induct)
+    apply(auto simp: Let_def)
+  done
+
+lemma is_normal_elim_NEq_Zero:
+  assumes "\<forall>a \<in> set es. is_Eq a \<longrightarrow> is_normal a"
+  assumes "\<forall>a \<in> set es. is_NEq a \<longrightarrow> (\<exists>x. a = NEq (Var x) Zero)"
+  shows "\<forall>a \<in> set (elim_NEq_Zero es). is_normal a"
+  using is_normal_elim_NEq_Zero_aux[OF assms] unfolding elim_NEq_Zero_def by blast
+
+lemma I_atom_Var_NEq_Zero_if_I_atom_Var_Eq_Succ:
+  "I_atom v (Eq (Var x) (Succ 1 (Var fx))) \<Longrightarrow> I_atom v (NEq (Var x) Zero)"
+  by simp
+
+lemma I_atom_if_I_atom_elim_NEq_Zero_aux:
+  assumes "\<forall>a \<in> set (elim_NEq_Zero_aux us es). I_atom v a"
+  shows "\<forall>a \<in> set es. I_atom v a"
+  using assms I_atom_Var_NEq_Zero_if_I_atom_Var_Eq_Succ
+  apply (induction us es rule: elim_NEq_Zero_aux.induct)
+        apply(auto simp: Let_def)
+  done
+
+lemma I_atom_if_I_atom_elim_NEq_Zero:
+  assumes "\<forall>a \<in> set (elim_NEq_Zero es). I_atom v a"
+  shows "\<forall>a \<in> set es. I_atom v a"
+  using assms I_atom_if_I_atom_elim_NEq_Zero_aux
+  unfolding elim_NEq_Zero_def by blast
+
+lemma aux:
+  assumes "I_atom v (NEq (Var x) Zero)" "x \<noteq> fx"
+  shows "I_atom (v(fx := nat.pred (v x))) (Eq (Var x) (Succ 1 (Var fx)))"
+  using assms by auto
+
+lemma I_term_if_eq_on_set_suc_term:
+  assumes "\<forall>x \<in> set_suc_term t. v' x = v x"
+  shows "I_term v' t = I_term v t"
+  using assms
+  apply(induction t)
+    apply(auto)
+  done
+
+lemma I_atom_if_eq_on_set_suc_atom:
+  assumes "\<forall>x \<in> set_suc_atom a. v' x = v x"
+  shows "I_atom v' a = I_atom v a"
+  using assms
+  apply (cases a)
+  apply(simp_all)
+   apply (metis I_term_if_eq_on_set_suc_term UnI1 UnI2)+
+  done
+
+lemma
+  assumes "finite us" "\<Union>(set_suc_atom ` set es) \<subseteq> us"
+  assumes "a \<in> set (elim_NEq_Zero_aux us es)"
+  assumes "x \<in> us"
+  shows "fresh us x \<notin> set_suc_atom a"
+  using assms
+proof(induction us es rule: elim_NEq_Zero_aux.induct)
+  case (1 uu)
+  then show ?case by simp
+next
+  case (2 us y es)
+  then have "fresh (insert (fresh us y) us) x \<notin> set_suc_atom a"
+    if "a \<in> set (elim_NEq_Zero_aux (insert (fresh us y) us) es)"
+    using that by (simp add: subset_insertI2)
+  from 2 have "set_suc_atom a \<subseteq> insert (fresh us y) us"
+        if "a \<in> set (elim_NEq_Zero_aux (insert (fresh us y) us) es)"
+    using that apply(auto) 
+  from "2"(2-) show ?case apply(simp) sorry
+qed (use fresh_notIn in \<open>force+\<close>)
+
+lemma
+  assumes "\<Union>(set_suc_atom ` set es) \<subseteq> us" "finite us"
+  assumes "\<forall>a \<in> set es. I_atom v a"
+  obtains v' where "\<forall>a \<in> set (elim_NEq_Zero_aux us es). I_atom v' a"
+                   "\<forall>x \<in> us. v' x = v x"
+  using assms
 (*
-inductive proves_suc :: "'a suc_atom set \<Rightarrow> 'a suc_atom \<Rightarrow> bool" (infix "\<turnstile>\<^bsub>Suc\<^esub>" 60) where
-  "a \<in> A \<Longrightarrow> A \<turnstile>\<^bsub>Suc\<^esub> a"
-| "A \<turnstile>\<^bsub>Suc\<^esub> Eq t t"
-| "A \<turnstile>\<^bsub>Suc\<^esub> Eq t1 t2 \<Longrightarrow> A \<turnstile>\<^bsub>Suc\<^esub> Eq t2 t1"
-| "A \<turnstile>\<^bsub>Suc\<^esub> NEq t1 t2 \<Longrightarrow> A \<turnstile>\<^bsub>Suc\<^esub> NEq t2 t1"
-| "A \<turnstile>\<^bsub>Suc\<^esub> Eq t1 t2 \<Longrightarrow> A \<turnstile>\<^bsub>Suc\<^esub> NEq t1 t2 \<Longrightarrow> A \<turnstile>\<^bsub>Suc\<^esub> NEq Zero Zero"
-| "A \<turnstile>\<^bsub>Suc\<^esub> Eq (Succ t1) (Succ t2) \<Longrightarrow> A \<turnstile>\<^bsub>Suc\<^esub> Eq t1 t2"
-| "A \<turnstile>\<^bsub>Suc\<^esub> Eq (Var x) t \<Longrightarrow> A \<turnstile>\<^bsub>Suc\<^esub> a
-  \<Longrightarrow> A \<turnstile>\<^bsub>Suc\<^esub> subst_suc_atom (\<lambda>y. if x = y then t else Var y) a"
+proof(induction es arbitrary: us thesis)
+  case Nil
+  then show ?case sorry
+next
+  case (Cons e es)
+  consider
+    x where "e = NEq (Var x) Zero" | "\<forall>x. e \<noteq> NEq (Var x) Zero"
+    by blast
+  then show ?case
+  proof cases
+    case 1
+    then show ?thesis sorry
+  next
+    case 2
+    then show ?thesis sorry
+  qed
+qed
 *)
+proof(induction us es arbitrary: thesis rule: elim_NEq_Zero_aux.induct)
+  case (1 us)
+  then show ?case  sorry
+next
+  case (2 us x es thesis)
+  then obtain v' where
+    v': "\<forall>a \<in> set (elim_NEq_Zero_aux (insert (fresh us x) us) es). I_atom v' a"
+        "\<forall>x \<in> insert (fresh us x) us. v' x = v x"
+    by (auto simp: subset_insertI2)
+  with "2.prems"(3) have "fresh us x \<notin> us" "\<forall>x \<in> us. (v'(fresh us x := nat.pred (v' x))) x = v x"
+    using fresh_notIn by (metis fun_upd_apply insertCI)+
+  moreover from "2.prems"(2) have "x \<in> us"
+    by auto
+  moreover from "2.prems"(4) have "v x \<noteq> 0"
+    by simp
+  with v' \<open>x \<in> us\<close> have "v' x \<noteq> 0"
+    by simp
+  ultimately show ?case apply(intro "2"(2)[where ?v'="v'(fresh us x := nat.pred (v' x))"])
+     apply(auto simp: Let_def) apply(metis)
+next
+  case ("3_1" us s t es)
+  then obtain v'
+    where v': "\<forall>a \<in> set (elim_NEq_Zero_aux us es). I_atom v' a"
+              "\<forall>x \<in> us. v' x = v x"
+    by auto
+  with "3_1" have "\<forall>x \<in> set_suc_atom (Eq s t). v x = v' x"
+    by auto
+  from I_atom_if_eq_on_set_suc_atom[OF this] have "I_atom v' (Eq s t) = I_atom v (Eq s t)"
+    by blast
+  with "3_1" v' show ?case
+    by simp
+next
+  case ("3_2" us va es)
+  then show ?case sorry
+next
+  case ("3_3" us vb vc va es)
+  then show ?case sorry
+next
+  case ("3_4" us v vb es)
+  then show ?case sorry
+next
+  case ("3_5" us v vb vc es)
+  then show ?case sorry
+qed
+
+hide_const (open) Var subst_term subst_atom is_normal I_term I_atom is_Eq is_NEq
 
 end
